Martin Escardo, 2014, 21 March 2018, November-December 2019.

The type Fin n is a discrete set with n elements.

 * The function Fin : ℕ → 𝓤₀ is left-cancellable, or an injection (but
   not an embedding in the sense of univalent mathematics).

 * Exhaustive search over Fin n, or its compactness, finding a minimal
   element with a decidable property.

 * m ≤ n iff there is an injection Fin m → Fin n.

 * Finite types, defined by the unspecified existence of an
   isomorphism with some Fin n.

 * Various forms of the pigeonhole principle, and its application to
   show that every element of a finite group has a finite order.

And more.

Other interesting uses of the types Fin n is in the file
https://www.cs.bham.ac.uk/~mhe/agda-new/ArithmeticViaEquivalence.html
which proves commutativity of addition and multiplication, and more,
using the corresponding property for (finite) types.

\begin{code}

{-# OPTIONS --without-K --exact-split --safe #-}

open import SpartanMLTT

module Fin  where

Fin : ℕ → 𝓤₀ ̇
Fin 0        = 𝟘
Fin (succ n) = Fin n + 𝟙

\end{code}

We have zero and successor for finite sets, with the following types:

\begin{code}

fzero : {n : ℕ} → Fin (succ n)
fzero = inr *

fsucc : {n : ℕ} → Fin n → Fin (succ n)
fsucc = inl

\end{code}

But it will more convenient to have them as patterns, for the sake of
clarity in definitions by pattern matching:

\begin{code}

pattern 𝟎     = inr *
pattern suc i = inl i

\end{code}

The induction principle for Fin is proved by induction on ℕ:

\begin{code}

Fin-induction : (P : (n : ℕ) → Fin n → 𝓤 ̇ )
              → ((n : ℕ) → P (succ n) 𝟎)
              → ((n : ℕ) (i : Fin n) → P n i → P (succ n) (suc i))
              →  (n : ℕ) (i : Fin n) → P n i

Fin-induction P β σ 0        i       = 𝟘-elim i
Fin-induction P β σ (succ n) 𝟎       = β n
Fin-induction P β σ (succ n) (suc i) = σ n i (Fin-induction P β σ n i)

\end{code}

We will not use this induction principle explicitly. Instead, we will
use the above pattern for similar definitions by induction.

The left cancellability of Fin uses the construction +𝟙-cancellable
defined in the module PlusOneLC.lagda.

\begin{code}

open import PlusOneLC
open import UF-Equiv

Fin-lc : (m n : ℕ) → Fin m ≃ Fin n → m ≡ n
Fin-lc 0           0       p = refl
Fin-lc (succ m)    0       p = 𝟘-elim (⌜ p ⌝ 𝟎)
Fin-lc 0          (succ n) p = 𝟘-elim (⌜ ≃-sym p ⌝ 𝟎)
Fin-lc (succ m)   (succ n) p = ap succ r
 where
  IH : Fin m ≃ Fin n → m ≡ n
  IH = Fin-lc m n

  remark : Fin m + 𝟙 ≃ Fin n + 𝟙
  remark = p

  q : Fin m ≃ Fin n
  q = +𝟙-cancellable p

  r : m ≡ n
  r = IH q

\end{code}

Notice that Fin is an example of a map that is left-cancellable but
not an embedding in the sense of univalent mathematics.

Recall that a type is discrete if it has decidable equality.

\begin{code}

open import DiscreteAndSeparated

Fin-is-discrete : (n : ℕ) → is-discrete (Fin n)
Fin-is-discrete 0        = 𝟘-is-discrete
Fin-is-discrete (succ n) = +discrete (Fin-is-discrete n) 𝟙-is-discrete

open import UF-Subsingletons
open import UF-Miscelanea

Fin-is-set : (n : ℕ) → is-set (Fin n)
Fin-is-set n = discrete-types-are-sets (Fin-is-discrete n)

\end{code}

Added November 2019. The type Fin n is compact, or exhaustively
searchable.

\begin{code}

open import CompactTypes

Fin-Compact : (n : ℕ) → Compact (Fin n) {𝓤}
Fin-Compact 0        = 𝟘-Compact
Fin-Compact (succ n) = +-Compact (Fin-Compact n) 𝟙-Compact


Fin-Π-Compact : (n : ℕ) → Π-Compact (Fin n) {𝓤}
Fin-Π-Compact n = Σ-Compact-gives-Π-Compact (Fin n) (Fin-Compact n)


Fin-Compact∙ : (n : ℕ) → Compact∙ (Fin (succ n)) {𝓤}
Fin-Compact∙ n = Compact-pointed-gives-Compact∙ (Fin-Compact (succ n)) 𝟎

\end{code}

Recall that X ↣ Y is the type of left cancellable maps from X to Y,
which should not be confused with the type X ↪ Y of embeddings of X
into Y. However, for types that are sets, like Fin n, there is no
difference between the embedding property and left cancellability.

\begin{code}

open import Plus-Properties
open import Swap
open import UF-LeftCancellable

+𝟙-cancel-lemma : {X Y : 𝓤 ̇}
                → (𝒇 : X + 𝟙 ↣ Y + 𝟙)
                → ⌈ 𝒇 ⌉ 𝟎 ≡ 𝟎
                → X ↣ Y

+𝟙-cancel-lemma {𝓤} {X} {Y} (f , l) p = g , m
 where
  g : X → Y
  g x = pr₁ (inl-preservation {𝓤} {𝓤} {𝓤} {𝓤} f p l x)

  a : (x : X) → f (suc x) ≡ suc (g x)
  a x = pr₂ (inl-preservation f p l x)

  m : left-cancellable g
  m {x} {x'} p = q
   where
    r = f (suc x)  ≡⟨ a x      ⟩
        suc (g x)  ≡⟨ ap suc p ⟩
        suc (g x') ≡⟨ (a x')⁻¹ ⟩
        f (suc x') ∎

    q : x ≡ x'
    q = inl-lc (l r)


+𝟙-cancel : {X Y : 𝓤 ̇}
          → is-discrete Y
          → X + 𝟙 ↣ Y + 𝟙
          → X ↣ Y

+𝟙-cancel {𝓤} {X} {Y} i (f , e) = a
 where
  h : Y + 𝟙 → Y + 𝟙
  h = swap (f 𝟎) 𝟎 (+discrete i 𝟙-is-discrete (f 𝟎)) new-point-is-isolated

  d : left-cancellable h
  d = equivs-are-lc h (swap-is-equiv (f 𝟎) 𝟎 (+discrete i 𝟙-is-discrete (f 𝟎)) new-point-is-isolated)

  f' : X + 𝟙 → Y + 𝟙
  f' = h ∘ f

  e' : left-cancellable f'
  e' = left-cancellable-closed-under-∘ f h e d

  p : f' 𝟎 ≡ 𝟎
  p = swap-equation₀ (f 𝟎) 𝟎 (+discrete i 𝟙-is-discrete (f 𝟎)) new-point-is-isolated

  a : X ↣ Y
  a = +𝟙-cancel-lemma (f' , e') p

open import NaturalsOrder
open import UF-EquivalenceExamples

\end{code}

In set theory, natural numbers are defined as certain sets, and their
order relation is inherited from the ordering of sets defined by the
existence of injections, or left-cancellable maps. Here, in type
theory, we have defined m ≤ n by induction on m and n, in the style of
Peano Arithmetic, but we can prove that this relation is characterized
by this injection property:

\begin{code}

↣-gives-≤ : (m n : ℕ) → (Fin m ↣ Fin n) → m ≤ n
↣-gives-≤ 0        n        e       = zero-minimal n
↣-gives-≤ (succ m) 0        (f , i) = 𝟘-elim (f 𝟎)
↣-gives-≤ (succ m) (succ n) e       = ↣-gives-≤ m n (+𝟙-cancel (Fin-is-discrete n) e)


canonical-Fin-inclusion : (m n : ℕ) → m ≤ n → (Fin m → Fin n)
canonical-Fin-inclusion 0        n        l = unique-from-𝟘
canonical-Fin-inclusion (succ m) 0        l = 𝟘-elim l
canonical-Fin-inclusion (succ m) (succ n) l = +functor IH unique-to-𝟙
 where
  IH : Fin m → Fin n
  IH = canonical-Fin-inclusion m n l


canonical-Fin-inclusion-lc : (m n : ℕ) (l : m ≤ n)
                           → left-cancellable (canonical-Fin-inclusion m n l)

canonical-Fin-inclusion-lc 0        n        l {x}     {y}     p = 𝟘-elim x
canonical-Fin-inclusion-lc (succ m) 0        l {x}     {y}     p = 𝟘-elim l
canonical-Fin-inclusion-lc (succ m) (succ n) l {suc x} {suc y} p = γ
 where
  IH : canonical-Fin-inclusion m n l x ≡ canonical-Fin-inclusion m n l y → x ≡ y
  IH = canonical-Fin-inclusion-lc m n l

  γ : suc x ≡ suc y
  γ = ap suc (IH (inl-lc p))

canonical-Fin-inclusion-lc (succ m) (succ n) l {𝟎} {𝟎} p = refl


≤-gives-↣ : (m n : ℕ) → m ≤ n → (Fin m ↣ Fin n)
≤-gives-↣ m n l = canonical-Fin-inclusion m n l , canonical-Fin-inclusion-lc m n l

\end{code}

An equivalent, shorter construction:

\begin{code}
≤-gives-↣' : (m n : ℕ) → m ≤ n → (Fin m ↣ Fin n)
≤-gives-↣' 0        n        l = unique-from-𝟘 , (λ {x} {x'} p → 𝟘-elim x)
≤-gives-↣' (succ m) 0        l = 𝟘-elim l
≤-gives-↣' (succ m) (succ n) l = g , j
 where
  IH : Fin m ↣ Fin n
  IH = ≤-gives-↣' m n l

  f : Fin m → Fin n
  f = pr₁ IH

  i : left-cancellable f
  i = pr₂ IH

  g : Fin (succ m) → Fin (succ n)
  g = +functor f unique-to-𝟙

  j : left-cancellable g
  j {suc x} {suc x'} p = ap suc (i (inl-lc p))
  j {suc x} {𝟎}      p = 𝟘-elim (+disjoint  p)
  j {𝟎}     {suc y}  p = 𝟘-elim (+disjoint' p)
  j {𝟎}     {𝟎}      p = refl

\end{code}

Added 9th December 2019. A version of the pigeonhole principle, which
uses (one direction of) the above characterization of the relation m ≤ n
as the existence of an injection Fin m → Fin n:

\begin{code}

_has-a-repetition : {X : 𝓤 ̇ } {Y : 𝓥 ̇ } → (X → Y) → 𝓤 ⊔ 𝓥 ̇
f has-a-repetition = Σ x ꞉ domain f , Σ x' ꞉ domain f , (x ≢ x') × (f x ≡ f x')


pigeonhole-principle : (m n : ℕ) (f : Fin m → Fin n)
                     → m > n → f has-a-repetition
pigeonhole-principle m n f g = γ
 where
  a : ¬ (Σ f ꞉ (Fin m → Fin n), left-cancellable f)
  a = contrapositive (↣-gives-≤ m n) (less-not-bigger-or-equal n m g)

  b : ¬ left-cancellable f
  b l = a (f , l)

  c : ¬ ((i j : Fin m) → f i ≡ f j → i ≡ j)
  c φ = b (λ {i} {j} → φ i j)

  d : ¬¬ (f has-a-repetition)
  d ψ = c δ
   where
    ε : (i j : Fin m) → f i ≡ f j → ¬(i ≢ j)
    ε i j p ν = ψ (i , j , ν , p)
    δ : (i j : Fin m) → f i ≡ f j → i ≡ j
    δ i j p = ¬¬-elim (Fin-is-discrete m i j) (ε i j p)

\end{code}

A classical proof ends at this point. For a constructive proof, we
need more steps.

\begin{code}

  u : (i j : Fin m) → decidable ((i ≢ j) × (f i ≡ f j))
  u i j = ×-preserves-decidability
           (¬-preserves-decidability (Fin-is-discrete m i j))
           (Fin-is-discrete n (f i) (f j))

  v : (i : Fin m) → decidable (Σ j ꞉ Fin m , (i ≢ j) × (f i ≡ f j))
  v i = Fin-Compact m _ (u i)

  w : decidable (f has-a-repetition)
  w = Fin-Compact m _ v

  γ : f has-a-repetition
  γ = ¬¬-elim w d

\end{code}

This, of course, doesn't give the most efficient algorithm, but it
does give an algorithm for computing an argument of the function whose
value is repeated.

Added 2nd December 2019. An isomorphic copy of the type Fin n:

\begin{code}

Fin' : ℕ → 𝓤₀ ̇
Fin' n = Σ k ꞉ ℕ , k < n


𝟎' : {n : ℕ} → Fin' (succ n)
𝟎' {n} = 0 , zero-minimal n


suc' : {n : ℕ} → Fin' n → Fin' (succ n)
suc' (k , l) = succ k , l


Fin-unprime : (n : ℕ) → Fin' n → Fin n
Fin-unprime 0        (k , l)      = 𝟘-elim l
Fin-unprime (succ n) (0 , l)      = 𝟎
Fin-unprime (succ n) (succ k , l) = suc (Fin-unprime n (k , l))


Fin-prime : (n : ℕ) → Fin n → Fin' n
Fin-prime 0        i       = 𝟘-elim i
Fin-prime (succ n) (suc i) = suc' (Fin-prime n i)
Fin-prime (succ n) 𝟎       = 𝟎'

ηFin : (n : ℕ) → Fin-prime n ∘ Fin-unprime n ∼ id
ηFin 0        (k , l)      = 𝟘-elim l
ηFin (succ n) (0 , *)      = refl
ηFin (succ n) (succ k , l) = ap suc' (ηFin n (k , l))


εFin : (n : ℕ) → Fin-unprime n ∘ Fin-prime n ∼ id
εFin 0        i       = 𝟘-elim i
εFin (succ n) (suc i) = ap suc (εFin n i)
εFin (succ n) 𝟎       = refl


Fin-prime-is-equiv : (n : ℕ) → is-equiv (Fin-prime n)
Fin-prime-is-equiv n = qinvs-are-equivs (Fin-prime n) ((Fin-unprime n) , εFin n , ηFin n)


≃-Fin : (n : ℕ) → Fin n ≃ Fin' n
≃-Fin n = Fin-prime n , Fin-prime-is-equiv n

\end{code}

Added 10th Dec 2019. We define the natural order of Fin n by reduction
to the natural order of ℕ so that the canonical embedding Fin n → ℕ is
order preserving and reflecting, using the above isomorphic
manifestation of the type Fin n.

\begin{code}

open import NaturalNumbers-Properties

Fin↦ℕ : {n : ℕ} → Fin n → ℕ
Fin↦ℕ {n} = pr₁ ∘ Fin-prime n


Fin↦ℕ-property : {n : ℕ} (i : Fin n) → Fin↦ℕ i < n
Fin↦ℕ-property {n} i = pr₂ (Fin-prime n i)

open import UF-Embeddings

Fin↦ℕ-is-embedding : (n : ℕ) → is-embedding (Fin↦ℕ {n})
Fin↦ℕ-is-embedding n = ∘-is-embedding
                        (equivs-are-embeddings (Fin-prime n) (Fin-prime-is-equiv n))
                        (pr₁-is-embedding (λ i → <-is-prop-valued i n))


Fin↦ℕ-lc : (n : ℕ) → left-cancellable (Fin↦ℕ {n})
Fin↦ℕ-lc n = embeddings-are-left-cancellable Fin↦ℕ (Fin↦ℕ-is-embedding n)


_≺_ _≼_ : {n : ℕ} → Fin n → Fin n → 𝓤₀ ̇
i ≺ j = Fin↦ℕ i < Fin↦ℕ j
i ≼ j = Fin↦ℕ i ≤ Fin↦ℕ j


_is-lower-bound-of_ : {n : ℕ} → Fin n → (Fin n → 𝓤 ̇ ) → 𝓤 ̇
i is-lower-bound-of A = ∀ j → A j → i ≼ j


lower-bounds-of : {n : ℕ} → (Fin n → 𝓤 ̇ ) → Fin n → 𝓤 ̇
lower-bounds-of A = λ i → i is-lower-bound-of A


_is-upper-bound-of_ : {n : ℕ} → Fin n → (Fin n → 𝓤 ̇ )  → 𝓤 ̇
i is-upper-bound-of A = ∀ j → A j → j ≼ i


_is-inf-of_ : {n : ℕ} → Fin n → (Fin n → 𝓤 ̇ ) → 𝓤 ̇
i is-inf-of A = i is-lower-bound-of A
              × i is-upper-bound-of (lower-bounds-of A)


inf-is-lb : {n : ℕ} (i : Fin n) (A : Fin n → 𝓤 ̇ )
          → i is-inf-of A → i is-lower-bound-of A

inf-is-lb i A = pr₁


inf-is-ub-of-lbs : {n : ℕ} (i : Fin n) (A : Fin n → 𝓤 ̇ )
                 → i is-inf-of A → i is-upper-bound-of (lower-bounds-of A)

inf-is-ub-of-lbs i A = pr₂


inf-construction : {n : ℕ} (A : Fin (succ n) → 𝓤 ̇ )
                 → detachable A
                 → Σ i ꞉ Fin (succ n) , i is-inf-of A × (Σ A → A i)

inf-construction {𝓤} {zero} A δ = 𝟎 , (l , m) , ε
 where
  l : 𝟎 is-lower-bound-of A
  l 𝟎       _ = ≤-refl 0
  l (suc i) _ = 𝟘-elim i

  m : (j : Fin 1) → j is-lower-bound-of A → j ≼ 𝟎
  m 𝟎       _ = ≤-refl 0
  m (suc i) _ = 𝟘-elim i

  ε : Σ A → A 𝟎
  ε (𝟎 , a)     = a
  ε (suc i , a) = 𝟘-elim i

inf-construction {𝓤} {succ n} A δ = γ (δ 𝟎)
 where
  IH : Σ i ꞉ Fin (succ n) , i is-inf-of (A ∘ suc) × ((Σ j ꞉ Fin (succ n) , A (suc j)) → A (suc i))
  IH = inf-construction {𝓤} {n} (A ∘ suc) (δ ∘ suc)

  i : Fin (succ n)
  i = pr₁ IH

  l : (j : Fin (succ n)) → A (suc j) → i ≼ j
  l = inf-is-lb i (A ∘ suc) (pr₁ (pr₂ IH))

  u : (j : Fin (succ n)) → ((k : Fin (succ n)) → A (suc k) → j ≼ k) → j ≼ i
  u = inf-is-ub-of-lbs i (A ∘ suc) (pr₁ (pr₂ IH))

  γ : decidable (A 𝟎) → Σ i' ꞉ Fin (succ (succ n)) , i' is-inf-of A × (Σ A → A i')
  γ (suc a) = 𝟎 , (φ , ψ) , ε
    where
     φ : (j : Fin (succ (succ n))) → A j → 𝟎 ≼ j
     φ j b = zero-minimal (Fin↦ℕ j)

     ψ : (j : Fin (succ (succ n))) → j is-lower-bound-of A → j ≼ 𝟎
     ψ j l = l 𝟎 a

     ε : Σ A → A 𝟎
     ε _ = a

  γ (inr ν) = suc i , (φ , ψ) , ε
    where
     φ : (j : Fin (succ (succ n))) → A j → suc i ≼ j
     φ 𝟎 a = 𝟘-elim (ν a)
     φ (suc j) a = l j a

     ψ : (j : Fin (succ (succ n))) → j is-lower-bound-of A → j ≼ suc i
     ψ 𝟎 l = zero-minimal (Fin↦ℕ i)
     ψ (suc j) l = u j (l ∘ suc)

     ε : Σ A → A (suc i)
     ε (𝟎 , b)     = 𝟘-elim (ν b)
     ε (suc j , b) = pr₂ (pr₂ IH) (j , b)


inf : {n : ℕ} (A : Fin (succ n) → 𝓤 ̇ ) → detachable A → Fin (succ n)
inf A δ = pr₁ (inf-construction A δ)


inf-property : {n : ℕ} (A : Fin (succ n) → 𝓤 ̇ ) (δ : detachable A)
             → (inf A δ) is-inf-of A

inf-property A δ = pr₁ (pr₂ (inf-construction A δ))


inf-is-attained : {n : ℕ} (A : Fin (succ n) → 𝓤 ̇ ) (δ : detachable A)
                → Σ A → A (inf A δ)

inf-is-attained A δ = pr₂ (pr₂ (inf-construction A δ))


Σₘᵢₙ : {n : ℕ} → (Fin n → 𝓤 ̇ ) → 𝓤 ̇
Σₘᵢₙ {𝓤} {n} A = Σ i ꞉ Fin n , A i × (i is-lower-bound-of A)


Σₘᵢₙ-gives-Σ : {n : ℕ} (A : Fin n → 𝓤 ̇ )
             → Σₘᵢₙ A → Σ A

Σₘᵢₙ-gives-Σ A (i , a , _) = (i , a)


Σ-gives-Σₘᵢₙ : {n : ℕ} (A : Fin n → 𝓤 ̇ )
             → detachable A → Σ A → Σₘᵢₙ A

Σ-gives-Σₘᵢₙ {𝓤} {0}      A δ (i , a) = 𝟘-elim i
Σ-gives-Σₘᵢₙ {𝓤} {succ n} A δ σ       = inf A δ ,
                                        inf-is-attained A δ σ ,
                                        inf-is-lb (inf A δ) A (inf-property A δ)


¬¬Σ-gives-Σₘᵢₙ : {n : ℕ} (A : Fin n → 𝓤 ̇ )
               → detachable A → ¬¬ Σ A → Σₘᵢₙ A

¬¬Σ-gives-Σₘᵢₙ {𝓤} {n} A δ u = Σ-gives-Σₘᵢₙ A δ (¬¬-elim (Fin-Compact n A δ) u)


is-prop-valued : {X : 𝓤 ̇ } → (X → 𝓥 ̇ ) → 𝓤 ⊔ 𝓥 ̇
is-prop-valued A = ∀ x → is-prop (A x)

open import UF-FunExt
open import UF-Subsingletons-FunExt
open import UF-Base

Σₘᵢₙ-is-prop : FunExt
             → {n : ℕ} (A : Fin n → 𝓤 ̇ )
             → is-prop-valued A → is-prop (Σₘᵢₙ A)

Σₘᵢₙ-is-prop {𝓤} fe {n} A h (i , a , l) (i' , a' , l') = γ
 where
  p : i ≡ i'
  p = Fin↦ℕ-lc n (≤-anti (Fin↦ℕ i) (Fin↦ℕ i') u v)
   where
    u : i ≼ i'
    u = l i' a'

    v : i' ≼ i
    v = l' i a

  H : ∀ j → is-prop (A j × (j is-lower-bound-of A))
  H j = ×-is-prop
         (h j)
         (Π-is-prop (fe 𝓤₀ 𝓤)
           (λ k → Π-is-prop (fe 𝓤 𝓤₀)
                   (λ b → ≤-is-prop-valued (Fin↦ℕ j) (Fin↦ℕ k))))

  γ : i , a , l ≡ i' , a' , l'
  γ = to-Σ-≡ (p , H _ _ _)

\end{code}

Added 8th December 2019. One defines a type to be finite, in univalent
mathematics, if it is isomorphic to Fin n for some n. But one has to
careful to express this, if we want finiteness to be property rather
than structure, with a suitably chosen notion of existence.

The following is structure rather than property. It amounts to the
type of finite linear orders on X.

\begin{code}

Finite : 𝓤 ̇ → 𝓤 ̇
Finite X = Σ n ꞉ ℕ , X ≃ Fin n

\end{code}

Exercise: If X ≃ Fin n, then the type Finite X has n! elements.

Hence one considers the following notion of finiteness, which is
property rather than structure:

\begin{code}

open import UF-PropTrunc

module finiteness (pt : propositional-truncations-exist) where

 open PropositionalTruncation pt public

 is-finite : 𝓤 ̇ → 𝓤 ̇
 is-finite X = Σ n ꞉ ℕ , ∥ X ≃ Fin n ∥


 cardinality : (X : 𝓤 ̇ ) → is-finite X → ℕ
 cardinality X = pr₁


 cardinality-≃ : (X : 𝓤 ̇ ) (φ : is-finite X) → ∥ X ≃ Fin (cardinality X φ) ∥
 cardinality-≃ X = pr₂


 being-finite-is-a-prop : (X : 𝓤 ̇ ) → is-prop (is-finite X)
 being-finite-is-a-prop X (m , d) (n , e) = γ
  where
   a : (m n : ℕ) → X ≃ Fin m → X ≃ Fin n → m ≡ n
   a m n d e = Fin-lc m n (≃-sym d ● e)

   b : (m n : ℕ) → ∥ X ≃ Fin m ∥ → ∥ X ≃ Fin n ∥ → m ≡ n
   b m n = ∥∥-rec₂ ℕ-is-set (a m n)

   γ : m , d ≡ n , e
   γ = to-Σ-≡ (b m n d e , ∥∥-is-a-prop _ _)

\end{code}

Equivalently, one can define finiteness as follows:

\begin{code}

 is-finite' : 𝓤 ̇ → 𝓤 ̇
 is-finite' X = ∃ n ꞉ ℕ , X ≃ Fin n


 being-finite'-is-a-prop : (X : 𝓤 ̇ ) → is-prop (is-finite' X)
 being-finite'-is-a-prop X = ∥∥-is-a-prop


 finite-unprime : (X : 𝓤 ̇ ) → is-finite' X → is-finite X
 finite-unprime X = ∥∥-rec (being-finite-is-a-prop X) γ
  where
   γ : (Σ n ꞉ ℕ , X ≃ Fin n) → Σ n ꞉ ℕ , ∥ X ≃ Fin n ∥
   γ (n , e) = n , ∣ e ∣


 finite-prime : (X : 𝓤 ̇ ) → is-finite X → is-finite' X
 finite-prime X (n , s) = ∥∥-rec ∥∥-is-a-prop (λ e → ∣ n , e ∣) s

\end{code}

Finite types are compact, or exhaustively searchable.

\begin{code}

 open CompactTypesPT pt

 finite-∥Compact∥ : {X : 𝓤 ̇ } → is-finite X → ∥ Compact X {𝓥} ∥
 finite-∥Compact∥ {𝓤} {𝓥} {X} (n , α) =
  ∥∥-functor (λ (e : X ≃ Fin n) → Compact-closed-under-≃ (≃-sym e) (Fin-Compact n)) α


 finite-∃-compact : FunExt → {X : 𝓤 ̇ } → is-finite X → ∃-Compact X {𝓥}
 finite-∃-compact fe φ = ∥Compact∥-gives-∃-Compact fe (finite-∥Compact∥ φ)

\end{code}

Finite types are discrete and hence sets:

\begin{code}

 finite-types-are-discrete : FunExt → {X : 𝓤 ̇ } → is-finite X → is-discrete X
 finite-types-are-discrete fe {X} (n , s) = ∥∥-rec (being-discrete-is-a-prop fe) γ s
  where
   γ : X ≃ Fin n → is-discrete X
   γ (f , e) = lc-maps-reflect-discreteness f (equivs-are-lc f e) (Fin-is-discrete n)


 finite-types-are-sets : FunExt → {X : 𝓤 ̇ } → is-finite X → is-set X
 finite-types-are-sets fe φ = discrete-types-are-sets (finite-types-are-discrete fe φ)

\end{code}

Example. The pigeonhole principle holds for finite types in the
following form:

\begin{code}

 finite-pigeonhole-principle : {X : 𝓤 ̇ } {Y : 𝓥 ̇ } (f : X → Y)
                               (φ : is-finite X) (ψ : is-finite Y)
                             → cardinality X φ > cardinality Y ψ
                             → ∥ f has-a-repetition ∥

 finite-pigeonhole-principle {𝓤} {𝓥} {X} {Y} f (m , s) (n , t) b = γ
  where
   h : Fin m ≃ X → Y ≃ Fin n → f has-a-repetition
   h (g , d) (h , e) = r r'
    where
     f' : Fin m → Fin n
     f' = h ∘ f ∘ g

     r' : f' has-a-repetition
     r' = pigeonhole-principle m n f' b

     r : f' has-a-repetition → f has-a-repetition
     r (i , j , u , p) = g i , g j , u' , p'
      where
       u' : g i ≢ g j
       u' = contrapositive (equivs-are-lc g d) u

       p' : f (g i) ≡ f (g j)
       p' = equivs-are-lc h e p

   γ : ∥ f has-a-repetition ∥
   γ = ∥∥-functor₂ h (∥∥-functor ≃-sym s) t

\end{code}

We now consider a situation in which anonymous existence gives
explicit existence:

\begin{code}

 Σₘᵢₙ-from-∃ : FunExt → {n : ℕ} (A : Fin n → 𝓤 ̇ )
             → detachable A → is-prop-valued A → ∃ A → Σₘᵢₙ A

 Σₘᵢₙ-from-∃ fe A δ h = ∥∥-rec (Σₘᵢₙ-is-prop fe A h) (Σ-gives-Σₘᵢₙ A δ)


 Fin-Σ-from-∃' : FunExt → {n : ℕ} (A : Fin n → 𝓤 ̇ )
               → detachable A → is-prop-valued A → ∃ A → Σ A

 Fin-Σ-from-∃' fe A δ h e = Σₘᵢₙ-gives-Σ A (Σₘᵢₙ-from-∃ fe A δ h e)

\end{code}

But the prop-valuedness of A is actually not needed, with more work:

\begin{code}

 Fin-Σ-from-∃ : FunExt → {n : ℕ} (A : Fin n → 𝓤 ̇ )
              → detachable A → ∃ A → Σ A

 Fin-Σ-from-∃ {𝓤} fe {n} A δ e = g σ'
  where
   A' : Fin n → 𝓤 ̇
   A' x = ∥ A x ∥

   δ' : detachable A'
   δ' x = d (δ x)
    where
     d : decidable (A x) → decidable (A' x)
     d (inl a) = inl ∣ a ∣
     d (inr u) = inr (∥∥-rec 𝟘-is-prop u)

   f : Σ A → Σ A'
   f (x , a) = x , ∣ a ∣

   e' : ∃ A'
   e' = ∥∥-functor f e

   σ' : Σ A'
   σ' = Fin-Σ-from-∃' fe A' δ' (λ x → ∥∥-is-a-prop) e'

   g : Σ A' → Σ A
   g (x , a') = x , ¬¬-elim (δ x) (λ (u : ¬ A x) → ∥∥-rec 𝟘-is-prop u a')

\end{code}

From now on we assume function extensionality:

\begin{code}

 module _ (fe : FunExt) where

\end{code}

We now consider further variations of the finite pigeonhole principle.

\begin{code}

  repeated-values : {X : 𝓤 ̇ } {Y : 𝓥 ̇ } → (X → Y) → X → 𝓤 ⊔ 𝓥 ̇
  repeated-values f x = Σ x' ꞉ domain f , (x ≢ x') × (f x ≡ f x')


  repetitions-detachable : {m : ℕ} {Y : 𝓥 ̇ } (f : Fin m → Y)
                         → is-finite Y
                         → detachable (repeated-values f)

  repetitions-detachable {𝓥} {m} {Y} f (n , t) i =
   Fin-Compact m
    (λ j → (i ≢ j) × (f i ≡ f j))
    (λ j → ×-preserves-decidability
            (¬-preserves-decidability (Fin-is-discrete m i j))
            (finite-types-are-discrete fe (n , t) (f i) (f j)))


  finite-pigeonhole-principle' : {m : ℕ} {Y : 𝓥 ̇ } (f : Fin m → Y)
                                 (ψ : is-finite Y)
                               → m > cardinality Y ψ
                               → f has-a-repetition

  finite-pigeonhole-principle' {𝓥} {m} {Y} f (n , t) b = γ
   where
    h : Y ≃ Fin n → f has-a-repetition
    h (h , e) = r r'
     where
      f' : Fin m → Fin n
      f' = h ∘ f

      r' : f' has-a-repetition
      r' = pigeonhole-principle m n f' b

      r : f' has-a-repetition → f has-a-repetition
      r (i , j , u , p) = i , j , u , equivs-are-lc h e p

    γ' : ∥ f has-a-repetition ∥
    γ' = ∥∥-functor h t

    A : Fin m → 𝓥 ̇
    A i = Σ j ꞉ Fin m , (i ≢ j) × (f i ≡ f j)

    γ : f has-a-repetition
    γ = Fin-Σ-from-∃ fe {m} A (repetitions-detachable f (n , t)) γ'

\end{code}

We can easily derive the construction finite-pigeonhole-principle from
finite-pigeonhole-principle', but at the expense of function
extensionality, which was not needed in our original construction.

Further versions of the pigeonhole principle are the following.

\begin{code}

  finite-pigeonhole-principle'' : {m : ℕ} {Y : 𝓥 ̇ } (f : Fin m → Y)
                                  (φ : is-finite Y)
                                → m > cardinality Y φ
                                → Σₘᵢₙ λ(i : Fin m) → repeated-values f i

  finite-pigeonhole-principle'' {𝓥} {m} {Y} f φ g =
   Σ-gives-Σₘᵢₙ
    (repeated-values f)
    (repetitions-detachable f φ)
    (finite-pigeonhole-principle' f φ g)


  ℕ-finite-pigeonhole-principle : {Y : 𝓥 ̇ } (f : ℕ → Y)
                                → is-finite Y
                                → f has-a-repetition

  ℕ-finite-pigeonhole-principle {𝓥} {Y} f (m , t) = r r'
   where
    f' : Fin (succ m) → Y
    f' i = f (Fin↦ℕ i)

    r' : f' has-a-repetition
    r' = finite-pigeonhole-principle' f'(m , t) (<-succ m)

    r : f' has-a-repetition → f has-a-repetition
    r (i , j , u , p) = Fin↦ℕ i , Fin↦ℕ j , contrapositive (Fin↦ℕ-lc (succ m)) u , p

\end{code}

Added 13th December 2019.

A well-known application of the pigeonhole principle is that every
element has a (minimal) finite order in a finite group. This holds
more generally for any finite type equipped with a left-cancellable
binary operation _·_ and a distinguished element e, with the same
construction.

\begin{code}

  module _ {X : 𝓤 ̇ }
           (φ : is-finite X)
           (_·_ : X → X → X)
           (lc : (x : X) → left-cancellable (x ·_))
           (e : X)
         where

    _↑_ : X → ℕ → X
    x ↑ 0        = e
    x ↑ (succ n) = x · (x ↑ n)

    infixl 3 _↑_

    finite-order : (x : X) → Σ k ꞉ ℕ , x ↑ (succ k) ≡ e
    finite-order x = c a
     where
      a : Σ m ꞉ ℕ , Σ n ꞉ ℕ , (m ≢ n) × (x ↑ m ≡ x ↑ n)
      a = ℕ-finite-pigeonhole-principle (x ↑_) φ

      b : (m : ℕ) (n : ℕ) → m ≢ n → x ↑ m ≡ x ↑ n → Σ k ꞉ ℕ , x ↑ (succ k) ≡ e
      b 0        0        ν p = 𝟘-elim (ν refl)
      b 0        (succ n) ν p = n , (p ⁻¹)
      b (succ m) 0        ν p = m , p
      b (succ m) (succ n) ν p = b m n (λ (q : m ≡ n) → ν (ap succ q)) (lc x p)

      c : type-of a → Σ k ꞉ ℕ , x ↑ (succ k) ≡ e
      c (m , n , ν , p) = b m n ν p

\end{code}

And of course then there is a minimal such k, by bounded minimization,
because finite types are discrete:

\begin{code}

    minimal-finite-order : (x : X) → Σμ λ(k : ℕ) → x ↑ (succ k) ≡ e
    minimal-finite-order x = minimal-from-given A γ (finite-order x)
     where
      A : ℕ → 𝓤 ̇
      A n = x ↑ (succ n) ≡ e

      γ : (n : ℕ) → decidable (x ↑ succ n ≡ e)
      γ n = finite-types-are-discrete fe φ (x ↑ succ n) e

\end{code}

Remark: the given construction finite-order already produces the
minimal order, but it seems slightly more difficult to prove this than
just compute the minimal order from any order. If we were interested
in the efficiency of our constructions (functional programs!), we
would have to consider this.

Added 15th December 2019.

If the type X i is compact for every i : Fin n, then the product type
(i : Fin n) → X i is also compact.

For that purpose we first consider generalized vector types.

\begin{code}

vec : (n : ℕ) → (Fin n → 𝓤 ̇ ) → 𝓤 ̇
vec 0        X = 𝟙
vec (succ n) X = X 𝟎 × vec n (X ∘ suc)

Vec : 𝓤 ̇ → (n : ℕ) → 𝓤 ̇
Vec X n = vec n (λ _ → X)

\end{code}

A version of the desired compactness construction:

\begin{code}

finite-product-compact : (n : ℕ) (X : Fin n → 𝓤 ̇ )
                       → ((i : Fin n) → Compact (X i) {𝓤})
                       → Compact (vec n X) {𝓤}

finite-product-compact zero     X c = 𝟙-Compact
finite-product-compact (succ n) X c = ×-Compact
                                       (c 𝟎)
                                       (finite-product-compact n (X ∘ suc) (c ∘ suc))

\end{code}

Standard operations on (generalized) vectors:

\begin{code}

pattern []       = *
pattern _∷_ x xs = (x , xs)


hd : {n : ℕ} {X : Fin (succ n) → 𝓤 ̇ } → vec (succ n) X → X 𝟎
hd (x ∷ xs) = x


tl : {n : ℕ} {X : Fin (succ n) → 𝓤 ̇ } → vec (succ n) X → vec n (X ∘ suc)
tl (x ∷ xs) = xs

index : (n : ℕ) {X : Fin n → 𝓤 ̇ } → vec n X → (i : Fin n) → X i
index 0        xs       i       = 𝟘-elim i
index (succ n) (x ∷ xs) 𝟎       = x
index (succ n) (x ∷ xs) (suc i) = index n xs i


_!!_ : {n : ℕ} {X : Fin n → 𝓤 ̇ } → vec n X → (i : Fin n) → X i
_!!_ {𝓤} {n} = index n

\end{code}

An isomorphic copy of vec n X.

\begin{code}

vec' : (n : ℕ) → (Fin n → 𝓤 ̇ ) → 𝓤 ̇
vec' n X = (i : Fin n) → X i


Vec' : 𝓤 ̇ → (n : ℕ) → 𝓤 ̇
Vec' X n = vec' n (λ _ → X)


hd' : {n : ℕ} {X : Fin (succ n) → 𝓤 ̇ } → vec' (succ n) X → X 𝟎
hd' xs = xs 𝟎


tl' : {n : ℕ} {X : Fin (succ n) → 𝓤 ̇ } → vec' (succ n) X → vec' n (X ∘ suc)
tl' xs = λ i → xs (suc i)


[]' : {X : Fin 0 → 𝓤 ̇ } → vec' 0 X
[]' = λ i → unique-from-𝟘 i


_∷'_ : {n : ℕ} {X : Fin (succ n) → 𝓤 ̇ } → X 𝟎 → vec' n (X ∘ suc) → vec' (succ n) X
(x ∷' xs) 𝟎       = x
(x ∷' xs) (suc i) = xs i


xedni : (n : ℕ) {X : Fin n → 𝓤 ̇ } → ((i : Fin n) → X i) → vec n X
xedni 0        xs' = []
xedni (succ n) xs' = hd' xs' ∷ xedni n (tl' xs')


vecη : (n : ℕ) {X : Fin n → 𝓤 ̇ } → xedni n {X} ∘ index n {X} ∼ id
vecη zero     []       = refl
vecη (succ n) (x ∷ xs) = ap (x ∷_) (vecη n xs)


module _ {𝓤} (fe : funext 𝓤₀ 𝓤) where

 vecε : (n : ℕ) {X : Fin n → 𝓤 ̇ } → index n {X} ∘ xedni n {X} ∼ id
 vecε 0        xs' = dfunext fe (λ i → 𝟘-elim i)
 vecε (succ n) xs' = dfunext fe h
  where
   h : (i : Fin (succ n)) → index (succ n) (xs' 𝟎 ∷ xedni n (tl' xs')) i ≡ xs' i
   h 𝟎       = refl
   h (suc i) = happly (vecε n (tl' xs')) i


 vec-≃ : (n : ℕ) {X : Fin n → 𝓤 ̇ } → vec n X ≃ vec' n X
 vec-≃ n {X} = qinveq (index n) (xedni n {X} , vecη n , vecε n)

\end{code}

The desired compactness theorem:

\begin{code}

 finitely-indexed-product-compact : (n : ℕ) (X : Fin n → 𝓤 ̇ )
                                  → ((i : Fin n) → Compact (X i))
                                  → Compact ((i : Fin n) → X i)

 finitely-indexed-product-compact n X c = Compact-closed-under-≃
                                           (vec-≃ n)
                                           (finite-product-compact n X c)

\end{code}
